proofs/lean/treehash-equivalence/Treehash.lean
@@ -1,5 +1,4 @@
 import Treehash.Basic
 import Treehash.Recursive
-import Treehash.IterLocal
-import Treehash.IterGlobal
+import Treehash.Iter
 import Treehash.Theorems
